Prove specs for more slice operations (#218)
Covers many use cases of slice.slice as well as general specs for slice.copy and slice.append.

I also fixed the models for slice.copy and slice.append.

Also adds an "assume" library to golang/defn.

new/golang/theory/slice.v
@@ -3,7 +3,7 @@ From iris.algebra Require Import dfrac.
 From Perennial.iris_lib Require Import dfractional.
 From Perennial.goose_lang Require Import ipersist.
 From New.golang.defn Require Export slice.
-From New.golang.theory Require Export list mem exception loop typing primitive auto.
+From New.golang.theory Require Export list mem assume exception loop typing primitive auto.
 From Perennial Require Import base.
 
 Set Default Proof Using "Type".
@@ -16,9 +16,11 @@ Module slice.
 Definition slice_f (sl : slice.t) (t : go_type) (n1 n2 : u64) : slice.t :=
   slice.mk (sl.(slice.ptr_f) +ₗ[t] uint.Z n1) (word.sub n2 n1) (word.sub sl.(slice.cap_f) n1).
 
+Definition full_slice_f (sl : slice.t) (t : go_type) (n1 n2 n3 : u64) : slice.t :=
+  slice.mk (sl.(slice.ptr_f) +ₗ[t] uint.Z n1) (word.sub n2 n1) (word.sub n3 n1).
+
 Definition elem_ref_f (sl : slice.t) (t : go_type) (i : u64) : loc :=
   sl.(slice.ptr_f) +ₗ[t] (uint.Z i).
-
 End slice.
 
 Section defns_and_lemmas.
@@ -41,20 +43,46 @@ Context `{!IntoValTyped V t}.
 Implicit Type (vs : list V).
 Definition own_slice_cap_def (s : slice.t) : iProp Σ :=
   ⌜ uint.Z s.(slice.len_f) ≤ uint.Z s.(slice.cap_f) ⌝ ∗
-  [∗ list] i ∈ (seq (uint.nat s.(slice.len_f)) (uint.nat s.(slice.cap_f) - uint.nat s.(slice.len_f))),
-    (s.(slice.ptr_f) +ₗ[t] Z.of_nat i) ↦ (default_val V).
+(* Two notes about this definition. First, it is written using [own_slice] to
+get some reuse, though an intermediate array points-to would be more useful
+here. Second, the capacity has arbitrary values, which is often desirable,
+but there are some niche cases where code could be aware of the contents of the
+capacity (for example, when sub-slicing from a larger slice) - actually taking
+advantage of that seems questionable though. *)
+  ∃ (vs: list V), own_slice
+                    (slice.mk
+                       (s.(slice.ptr_f) +ₗ[t] uint.Z s.(slice.len_f))
+                       (word.sub s.(slice.cap_f) s.(slice.len_f))
+                       (word.sub s.(slice.cap_f) s.(slice.len_f))) (DfracOwn 1) vs.
 Program Definition own_slice_cap := sealed @own_slice_cap_def.
 Definition own_slice_cap_unseal : own_slice_cap = _ := seal_eq _.
 
 Ltac unseal := rewrite ?own_slice_unseal /own_slice_def
                  ?own_slice_cap_unseal /own_slice_cap_def.
 
+Lemma own_slice_nil dq :
+  ⊢ slice.nil ↦*{dq} ([] : list V).
+Proof.
+  unseal. simpl. iPureIntro. split_and!; done.
+Qed.
+
+Lemma own_slice_empty dq s :
+  uint.Z s.(slice.len_f) = 0 ->
+  ⊢ s ↦*{dq} ([] : list V).
+Proof.
+  unseal. intros Hsz. destruct s. simpl in *.
+  iPureIntro. split_and!; [done|word|word].
+Qed.
+
 Lemma own_slice_cap_none s :
   s.(slice.len_f) = s.(slice.cap_f) →
   ⊢ own_slice_cap s.
 Proof.
-  destruct s; simpl; intros ->. rewrite own_slice_cap_unseal /own_slice_cap_def Nat.sub_diag //.
-  simpl. iPureIntro. lia.
+  destruct s; simpl; intros ->. rewrite own_slice_cap_unseal /own_slice_cap_def /=.
+  iSplit; [ done | ].
+  iExists [].
+  iApply own_slice_empty.
+  simpl. word.
 Qed.
 
 Lemma own_slice_len s dq vs :
@@ -62,9 +90,6 @@ Lemma own_slice_len s dq vs :
 Proof.
   unseal. iIntros "(_&[%%]) !% //".
 Qed.
-
-Lemma replicate_0 A (x:A) : replicate 0 x = [].
-Proof. reflexivity. Qed.
 
 #[global]
 Instance own_slice_dfractional s vs :
@@ -75,10 +100,7 @@ Instance own_slice_as_dfractional s dq vs :
   AsDFractional (s ↦*{dq} vs) (λ dq, s ↦*{dq} vs) dq.
 Proof. auto. Qed.
 
-Instance own_slice_fractional s vs :
-  fractional.Fractional (λ q, s ↦*{#q} vs).
-Proof. unseal; apply _. Qed.
-
+#[global]
 Instance own_slice_as_fractional s q vs :
   fractional.AsFractional (s ↦*{#q} vs) (λ q, s ↦*{#q} vs) q.
 Proof. unseal; split; auto; apply _. Qed.
@@ -86,19 +108,16 @@ Proof. unseal; split; auto; apply _. Qed.
 Lemma loc_add_stride_Sn l n :
   l +ₗ[t] S n = (l +ₗ go_type_size t) +ₗ[t] n.
 Proof.
-  replace (Z.mul (go_type_size t) (S n)) with (go_type_size t + Z.mul (go_type_size t) n).
-  { rewrite loc_add_assoc //. }
-  replace (Z.of_nat (S n)) with (1 + Z.of_nat n) by lia.
-  rewrite Z.mul_add_distr_l.
+  rewrite loc_add_assoc.
   f_equal.
-  rewrite Z.mul_1_r //.
+  lia.
 Qed.
 
 Lemma own_slice_agree s dq1 dq2 vs1 vs2 :
   s ↦*{dq1} vs1 -∗
   s ↦*{dq2} vs2 -∗
   ⌜vs1 = vs2⌝.
-Proof using Type*.
+Proof.
   unseal.
   iIntros "[Hs1 [%%]] [Hs2 [%%]]".
   assert (length vs1 = length vs2) by congruence.
@@ -163,27 +182,55 @@ Proof.
   iIntros "[? %]". naive_solver.
 Qed.
 
-Lemma own_slice_nil dq :
-  ⊢ slice.nil ↦*{dq} ([] : list V).
-Proof.
-  unseal. simpl. iPureIntro. split_and!; done.
-Qed.
-
-Lemma own_slice_empty dq s :
-  uint.Z s.(slice.len_f) = 0 ->
-  ⊢ s ↦*{dq} ([] : list V).
-Proof.
-  unseal. intros Hsz. destruct s. simpl in *.
-  iPureIntro. split_and!; [done|word|word].
-Qed.
-
 Lemma own_slice_cap_nil :
   ⊢ own_slice_cap slice.nil.
 Proof.
-  unseal. simpl. rewrite right_id.
-  rewrite (nil_length_inv (seq _ _)).
-  2:{ rewrite length_seq. word. }
-  simpl. word.
+  rewrite own_slice_cap_unseal /own_slice_cap_def /=.
+  iSplit; [ word | ].
+  iExists nil. iApply own_slice_empty.
+  reflexivity.
+Qed.
+
+Lemma slice_to_full_slice s n m :
+  slice.slice_f s t n m = slice.full_slice_f s t n m (slice.cap_f s).
+Proof. reflexivity. Qed.
+
+(* introduce a slice.slice_f for lemmas that require it *)
+Lemma slice_slice_trivial s :
+  s = slice.slice_f s t (W64 0) (slice.len_f s).
+Proof.
+  destruct s; simpl.
+  rewrite /slice.slice_f /=.
+  rewrite Z.mul_0_r loc_add_0.
+  f_equal; word.
+Qed.
+
+(* a variant of [slice_slice_trivial] that's easier to use with [iDestruct] and
+more discoverable with Search. *)
+Lemma own_slice_trivial_slice_f s dq (vs: list V) :
+  own_slice s dq vs ⊣⊢ own_slice (slice.slice_f s t (W64 0) (slice.len_f s)) dq vs.
+Proof.
+  rewrite -slice_slice_trivial //.
+Qed.
+
+Lemma own_slice_trivial_slice_f_2 s dq (vs: list V) :
+  own_slice (slice.slice_f s t (W64 0) (slice.len_f s)) dq vs ⊢ own_slice s dq vs.
+Proof.
+  rewrite -own_slice_trivial_slice_f //.
+Qed.
+
+Lemma slice_f_slice_f s n m n' m' :
+  uint.Z n + uint.Z n' < 2^64 →
+  uint.Z m' ≤ uint.Z m - uint.Z n →
+  slice.slice_f (slice.slice_f s t n m) t n' m' =
+    slice.slice_f s t (word.add n n') (word.add n m').
+Proof.
+  intros Hoverflow Hle.
+  rewrite /slice.slice_f /=.
+  rewrite !loc_add_assoc.
+  f_equal; try word.
+  rewrite -Z.mul_add_distr_l.
+  repeat (f_equal; try word).
 Qed.
 
 Lemma own_slice_elem_acc i v s dq vs :
@@ -240,6 +287,26 @@ Proof.
   { simpl. intros. f_equal. by erewrite IHn. }
 Qed.
 
+Lemma big_sepL_replicate_seq_general {PROP : bi} {A} (k n: nat) (v0: A) (P: nat → A → PROP) :
+  ([∗ list] i↦v ∈ replicate n v0, P (i + k)%nat v)%I = ([∗ list] i ∈ seq k n, P i v0)%I.
+Proof.
+  generalize dependent k.
+  induction n; auto; intros k.
+  simpl.
+  f_equal.
+  rewrite -IHn.
+  apply big_opL_ext => n' v Hget.
+  f_equal; lia.
+Qed.
+
+Lemma big_sepL_replicate_seq {PROP : bi} {A} (n: nat) (v0: A) (P: nat → A → PROP) :
+  ([∗ list] i↦v ∈ replicate n v0, P i v)%I = ([∗ list] i ∈ seq 0 n, P i v0)%I.
+Proof.
+  rewrite -big_sepL_replicate_seq_general.
+  apply big_opL_ext => n' v Hget.
+  f_equal; lia.
+Qed.
+
 Context `{!IntoVal V}.
 Context `{!IntoValTyped V t}.
 
@@ -270,11 +337,12 @@ Proof.
     wp_pures.
     rewrite slice_val_fold.
     iApply "HΦ".
-    rewrite own_slice_unseal own_slice_cap_unseal.
+    rewrite own_slice_unseal.
     assert (len = W64 0) by word; subst.
-    unfold own_slice_def. unfold own_slice_cap_def. simpl.
+    unfold own_slice_def. simpl.
     assert (uint.nat (W64 0) = 0)%nat as -> by word.
-    simpl. done.
+    simpl. iSplit; auto. iSplit; auto.
+    iApply own_slice_cap_none; reflexivity.
   }
   wp_pures.
   wp_bind (AllocN _ _).
@@ -317,12 +385,20 @@ Proof.
     rewrite default_val_eq_zero_val.
     erewrite has_go_type_len.
     2:{ apply zero_val_has_go_type. }
+    iExists (replicate (uint.nat cap - uint.nat len)%nat (default_val V)).
+    rewrite own_slice_unseal /own_slice_def /=.
+    iSplit; [ | len ].
+    rewrite big_sepL_replicate_seq.
+    rewrite (big_sepL_offset _ (uint.nat len)).
     iApply (big_sepL_impl with "[$]").
     iModIntro. iIntros.
     rewrite /pointsto_vals typed_pointsto_unseal /typed_pointsto_def /=.
     rewrite default_val_eq_zero_val.
     iApply (big_sepL_impl with "[$]").
-    iModIntro. iIntros. iFrame.
+    iModIntro. iIntros (???) "Hp". iExactEq "Hp".
+    rewrite !loc_add_assoc.
+    do 2 f_equal.
+    word.
   }
 Qed.
 
@@ -367,14 +443,421 @@ Proof.
   wp_call_lc "?". rewrite to_val_unseal. by iApply "HΦ".
 Qed.
 
-Global Instance wp_slice_elem_ref s (i : w64) :
+Global Instance pure_elem_ref s (i : w64) :
   PureWp (uint.Z i < uint.Z s.(slice.len_f)) (slice.elem_ref t #s #i)
     #(slice.elem_ref_f s t i).
 Proof.
   iIntros (?????) "HΦ".
-  wp_call.
+  wp_call_lc "?".
   rewrite bool_decide_true; last done.
-  wp_pure_lc "?". wp_pures. by iApply "HΦ".
+  wp_pures. by iApply "HΦ".
+Qed.
+
+Global Instance pure_slice_slice s (n m : w64) :
+  PureWp (uint.Z n ≤ uint.Z m ≤ uint.Z (slice.cap_f s) ∧
+          uint.Z (slice.len_f s) ≤ uint.Z (slice.cap_f s)) (slice.slice t #s #n #m)
+    #(slice.slice_f s t n m).
+Proof.
+  iIntros (?????) "HΦ".
+  wp_call_lc "?".
+  rewrite bool_decide_true; last word.
+  wp_pures.
+  rewrite bool_decide_true; last word.
+  wp_pures.
+  rewrite bool_decide_true; last word.
+  wp_pures.
+  iDestruct ("HΦ" with "[$]") as "HΦ".
+  iExactEq "HΦ".
+  repeat f_equal.
+  rewrite /slice.slice_f.
+  rewrite !to_val_unseal /=.
+  rewrite !to_val_unseal /=.
+  reflexivity.
+Qed.
+
+Global Instance pure_full_slice s (n m c : w64) :
+  PureWp (uint.Z n ≤ uint.Z m ≤ uint.Z c ∧
+          uint.Z c ≤ uint.Z (slice.cap_f s)) (slice.full_slice t #s #n #m #c)
+    #(slice.full_slice_f s t n m c).
+Proof.
+  iIntros (?????) "HΦ".
+  wp_call_lc "?".
+  rewrite bool_decide_true; last word.
+  wp_pures.
+  rewrite bool_decide_true; last word.
+  wp_pures.
+  rewrite bool_decide_true; last word.
+  wp_pures.
+  rewrite bool_decide_true; last word.
+  wp_pures.
+  iDestruct ("HΦ" with "[$]") as "HΦ".
+  iExactEq "HΦ".
+  repeat f_equal.
+  rewrite /slice.full_slice_f.
+  rewrite !to_val_unseal /=.
+  rewrite !to_val_unseal /=.
+  reflexivity.
+Qed.
+
+(** WP version of PureWp for discoverability and use with wp_apply.
+
+TODO: if PureWp instances had their pure side conditions dispatched with [word]
+this lemma would be pretty much unnecessary.
+*)
+Lemma wp_slice_slice_pure s (n m: w64) :
+  {{{ ⌜uint.Z n ≤ uint.Z m ≤ uint.Z s.(slice.cap_f) ∧
+        uint.Z s.(slice.len_f) ≤ uint.Z s.(slice.cap_f)⌝ }}}
+    slice.slice t #s #n #m
+  {{{ RET #(slice.slice_f s t n m); True }}}.
+Proof.
+  wp_start as "%".
+  wp_pure.
+  wp_pures.
+  iApply "HΦ". done.
+Qed.
+
+Lemma own_slice_split k s dq (vs: list V) n m :
+  uint.Z n ≤ uint.Z k ≤ uint.Z m →
+  slice.slice_f s t n m ↦*{dq} vs ⊣⊢
+  slice.slice_f s t n k ↦*{dq} take (uint.nat k - uint.nat n)%nat vs ∗
+  slice.slice_f s t k m ↦*{dq} drop (uint.nat k - uint.nat n)%nat vs.
+Proof.
+  intros Hle.
+  rewrite -{1}(take_drop (uint.nat k - uint.nat n)%nat vs).
+  rewrite own_slice_unseal /own_slice_def /=.
+  setoid_rewrite loc_add_assoc; setoid_rewrite <- Z.mul_add_distr_l.
+  rewrite big_sepL_app.
+  len.
+  replace (uint.nat (word.sub m n)) with (uint.nat m - uint.nat n)%nat by word.
+  iSplit.
+  - iIntros "((Hvs1 & Hvs2) & %Hwf)".
+    iSplitL "Hvs1".
+    + iSplit; [ | iPureIntro; move: Hwf; word ].
+      iFrame "Hvs1".
+    + iSplit; [ | iPureIntro; move: Hwf; word ].
+      iExactEq "Hvs2".
+      apply big_opL_ext => i v Hget.
+      do 3 f_equal.
+      word.
+  - iIntros "((Hvs1 & %Hwf1) & (Hvs2 & %Hwf2))".
+    iFrame "Hvs1".
+    iSplit; [ | iPureIntro; move: Hwf1 Hwf2; word ].
+    iExactEq "Hvs2".
+    apply big_opL_ext  => i v Hget.
+    do 3 f_equal.
+    move: Hwf1 Hwf2; word.
+Qed.
+
+Lemma own_slice_combine k s dq (vs1 vs2: list V) n m :
+  length vs1 = (uint.nat k - uint.nat n)%nat ∧
+  uint.Z n ≤ uint.Z k ≤ uint.Z m →
+  slice.slice_f s t n k ↦*{dq} vs1 -∗
+  slice.slice_f s t k m ↦*{dq} vs2 -∗
+  slice.slice_f s t n m ↦*{dq} (vs1 ++ vs2).
+Proof.
+  iIntros (Hwf) "Hs1 Hs2".
+  iApply (own_slice_split k).
+  { lia. }
+  rewrite -> take_app_le, take_ge by lia.
+  rewrite -> drop_app_le, drop_ge, app_nil_l by lia.
+  iFrame.
+Qed.
+
+Lemma own_slice_split_all k s dq (vs: list V) :
+  uint.Z k ≤ uint.Z s.(slice.len_f) →
+  s ↦*{dq} vs ⊣⊢
+  slice.slice_f s t (W64 0) k ↦*{dq} take (uint.nat k) vs ∗
+  slice.slice_f s t k s.(slice.len_f) ↦*{dq} drop (uint.nat k)%nat vs.
+Proof.
+  intros Hle.
+  rewrite {1}(own_slice_trivial_slice_f s).
+  rewrite -> (own_slice_split k) by word.
+  replace (uint.nat (W64 0)) with 0%nat by word.
+  replace (uint.nat k - 0)%nat with (uint.nat k) by lia.
+  auto.
+Qed.
+
+(* [own_slice_cap] only depends on where the end of the slice is *)
+Lemma own_slice_cap_same_end s s' :
+  slice.ptr_f s +ₗ[t] uint.Z (slice.len_f s) = slice.ptr_f s' +ₗ[t] uint.Z (slice.len_f s') →
+  uint.Z (slice.cap_f s) - uint.Z (slice.len_f s) = uint.Z (slice.cap_f s') - uint.Z (slice.len_f s') →
+  own_slice_cap V s ⊣⊢ own_slice_cap V s'.
+Proof.
+  intros Hend Hcap.
+  rewrite own_slice_cap_unseal /own_slice_cap_def.
+  assert (word.sub (slice.cap_f s) (slice.len_f s) = word.sub (slice.cap_f s') (slice.len_f s'))
+    as Hdiff by word.
+  rewrite -Hdiff.
+  rewrite -!Hend.
+  f_equiv.
+  iPureIntro; word.
+Qed.
+
+Lemma own_slice_cap_slice_f_change_first s n n' m :
+  uint.Z m ≤ uint.Z s.(slice.cap_f) ∧
+  uint.Z n ≤ uint.Z m ∧ uint.Z n' ≤ uint.Z m →
+  own_slice_cap V (slice.slice_f s t n m) ⊣⊢ own_slice_cap V (slice.slice_f s t n' m).
+Proof.
+  intros Hbound.
+  apply own_slice_cap_same_end; simpl.
+  - rewrite !loc_add_assoc -!Z.mul_add_distr_l.
+    repeat (f_equal; try word).
+  - word.
+Qed.
+
+Lemma own_slice_cap_slice_f s n :
+  uint.Z n ≤ uint.Z (slice.len_f s) ≤ uint.Z (slice.cap_f s) →
+  own_slice_cap V s ⊣⊢ own_slice_cap V (slice.slice_f s t n s.(slice.len_f)).
+Proof.
+  intros Hwf.
+  apply own_slice_cap_same_end; simpl.
+  - rewrite !loc_add_assoc -!Z.mul_add_distr_l.
+    repeat (f_equal; try word).
+  - word.
+Qed.
+
+(* Divide ownership of [s ↦* vs] around a slice [slice.slice_f s t n m].
+
+This is not the only choice; see [own_slice_f_cap] for a variation that uses
+capacity. *)
+Lemma own_slice_f (n m: w64) s dq (vs: list V) :
+  s ↦*{dq} vs ∗ ⌜uint.Z n ≤ uint.Z m ≤ uint.Z s.(slice.len_f)⌝ ⊢
+  (slice.slice_f s t (W64 0) n) ↦*{dq} (take (uint.nat n) vs) ∗
+  (slice.slice_f s t n m) ↦*{dq} (subslice (uint.nat n) (uint.nat m) vs) ∗
+  (* after the sliced part *)
+  (slice.slice_f s t m (slice.len_f s)) ↦*{dq} (drop (uint.nat m) vs).
+Proof.
+  iIntros "[Hs %]".
+  iDestruct (own_slice_len with "Hs") as %Hlen.
+  iDestruct (own_slice_wf with "Hs") as %Hwf.
+  iDestruct (own_slice_split_all n with "Hs") as "[Hs1 Hs2]".
+  { word. }
+  iDestruct (own_slice_split m with "Hs2") as "[Hs2 Hs3]";
+    [ move: Hlen; word | ].
+  iSplitL "Hs1".
+  { iExactEq "Hs1".
+    repeat (f_equal; try word). }
+  iSplitL "Hs2".
+  { iExactEq "Hs2".
+    rewrite subslice_drop_take; [ | word ].
+    repeat (f_equal; try word).  }
+  { iExactEq "Hs3".
+    rewrite drop_drop.
+    repeat (f_equal; try word). }
+Qed.
+
+Lemma own_slice_slice_absorb_capacity s (vs: list V) (n m: w64) :
+  uint.Z n ≤ uint.Z m ≤ uint.Z s.(slice.len_f) →
+  slice.slice_f s t m (slice.len_f s) ↦* vs ∗
+  own_slice_cap V s ⊢
+  own_slice_cap V (slice.slice_f s t n m).
+Proof.
+  iIntros (?) "[Hvs Hcap]".
+  iDestruct (own_slice_len with "Hvs") as %Hlen.
+  simpl in Hlen.
+  iDestruct (own_slice_wf with "Hvs") as %Hwf.
+  simpl in Hwf.
+  iDestruct (own_slice_cap_wf with "Hcap") as %Hwf'.
+  iApply (own_slice_cap_slice_f_change_first _ (W64 0)).
+  { word. }
+  rewrite own_slice_cap_unseal /own_slice_cap_def.
+  iDestruct "Hcap" as "[_ [%vs' Hvs']]".
+  iDestruct (own_slice_len with "Hvs'") as %Hlen'.
+  simpl in Hlen'.
+  simpl.
+  iSplit; [ word | ].
+  rewrite Z.mul_0_r loc_add_0 !word.sub_0_r.
+  iExists (vs ++ vs').
+  iApply (own_slice_split s.(slice.len_f)).
+  { word. }
+  rewrite -> take_app_le, take_ge by (move: Hlen Hlen'; word).
+  iFrame "Hvs".
+  rewrite -> drop_app_ge, drop_eq_0 by (move: Hlen Hlen'; word).
+  iFrame "Hvs'".
+Qed.
+
+(* divide ownership of [s ↦* vs ∗ own_slice_cap V s] around a slice [slice_f s t
+n m], moving ownership between m and [slice.len_f s] into the capacity of the
+slice *)
+Lemma own_slice_f_cap (n m: w64) s (vs: list V) :
+  s ↦* vs ∗ own_slice_cap V s ∗ ⌜uint.Z n ≤ uint.Z m ≤ uint.Z s.(slice.len_f)⌝ ⊢
+  (slice.slice_f s t (W64 0) n) ↦* (take (uint.nat n) vs) ∗
+  (slice.slice_f s t n m) ↦* (subslice (uint.nat n) (uint.nat m) vs) ∗
+  (* after the sliced part + capacity of original slice *)
+  own_slice_cap V (slice.slice_f s t n m).
+Proof.
+  iIntros "(Hs & Hcap & %)".
+  iDestruct (own_slice_len with "Hs") as %Hlen.
+  iDestruct (own_slice_f n m with "[$Hs]") as "(Hs1 & Hs2 & Hs3)".
+  { word. }
+  iFrame "Hs1 Hs2".
+  iDestruct (own_slice_slice_absorb_capacity with "[$Hs3 $Hcap]") as "$".
+  { word. }
+Qed.
+
+(** wp variant of [own_slice_f]
+
+TODO: try to avoid using this and use the canonical pure WP for slice.slice (plus directly using [own_slice_f])
+instead
+*)
+Lemma wp_slice_slice s dq (vs: list V) (n m : w64) :
+  {{{ s ↦*{dq} vs ∗ ⌜uint.Z n ≤ uint.Z m ≤ uint.Z s.(slice.len_f)⌝ }}}
+    slice.slice t #s #n #m
+  {{{ RET #(slice.slice_f s t n m);
+      (* before the sliced part *)
+      (slice.slice_f s t (W64 0) n) ↦*{dq} (take (uint.nat n) vs) ∗
+      (slice.slice_f s t n m) ↦*{dq} (subslice (uint.nat n) (uint.nat m) vs) ∗
+      (* after the sliced part *)
+      (slice.slice_f s t m (slice.len_f s)) ↦*{dq} (drop (uint.nat m) vs)
+  }}}.
+Proof.
+  wp_start as "[Hs %]".
+  iDestruct (own_slice_wf with "Hs") as %Hwf.
+  wp_apply wp_slice_slice_pure.
+  { word. }
+  iApply "HΦ".
+  iDestruct (own_slice_f n m with "[$Hs]") as "(Hs_pre & Hs & Hs_post)".
+  { word. }
+  iFrame.
+Qed.
+
+(** wp variant of [own_slice_f_cap]
+
+TODO: try to avoid using this and use the canonical pure WP for slice.slice (plus directly using [own_slice_f])
+instead
+*)
+Lemma wp_slice_slice_with_cap s (vs: list V) (n m : w64) :
+  {{{ s ↦* vs ∗ own_slice_cap V s ∗
+            ⌜uint.Z n ≤ uint.Z m ≤ uint.Z s.(slice.len_f)⌝ }}}
+    slice.slice t #s #n #m
+  {{{ RET #(slice.slice_f s t n m);
+      (* before the sliced part *)
+      (slice.slice_f s t (W64 0) n) ↦* (take (uint.nat n) vs) ∗
+      (slice.slice_f s t n m) ↦* (subslice (uint.nat n) (uint.nat m) vs) ∗
+      (* after the sliced part becomes part of this capacity *)
+      own_slice_cap V (slice.slice_f s t n m)
+  }}}.
+Proof.
+  wp_start as "(Hs & Hcap & %)".
+  iDestruct (own_slice_wf with "Hs") as %Hwf.
+  wp_apply wp_slice_slice_pure.
+  { word. }
+  iApply "HΦ".
+  iDestruct (own_slice_f_cap n m with "[$Hs $Hcap]") as "(Hs_pre & Hs & Hs_cap)".
+  { word. }
+  iFrame.
+Qed.
+
+Lemma own_slice_valid s dq (vs: list V) :
+  go_type_size t > 0 →
+  s ↦*{dq} vs ⊢ ⌜✓dq ∨ vs = []⌝.
+Proof.
+  iIntros (Hsize) "H".
+  destruct vs; [ by auto | ].
+  iLeft.
+  rewrite own_slice_unseal /own_slice_def.
+  simpl.
+  iDestruct "H" as "((H & _) & _)".
+  rewrite Z.mul_0_r loc_add_0.
+  iDestruct (typed_pointsto_valid with "H") as %Hvalid.
+  auto.
+Qed.
+
+(* An unusual use case for slicing where in s[n:m] we have len(s) ≤ m. This
+moves elements from the hidden capacity of s into its actual contents. *)
+Lemma own_slice_slice_into_capacity (n m: w64) s (vs: list V) :
+  s ↦* vs ∗ own_slice_cap V s ∗
+      ⌜uint.Z n ≤ uint.Z s.(slice.len_f) ≤ uint.Z m ≤ uint.Z s.(slice.cap_f)⌝ ⊢
+  ∃ (vs': list V),
+  (slice.slice_f s t (W64 0) n) ↦* (take (uint.nat n) vs) ∗
+      (slice.slice_f s t n m) ↦* (drop (uint.nat n) vs ++ vs') ∗
+      own_slice_cap V (slice.slice_f s t n m).
+Proof.
+  iIntros "(Hs & Hcap & %)".
+  iDestruct (own_slice_len with "Hs") as %Hlen.
+  iDestruct (own_slice_wf with "Hs") as %Hwf.
+  rewrite own_slice_cap_unseal /own_slice_cap_def /=.
+  iDestruct "Hcap" as "[_ [%vs' Hcap]]".
+  iDestruct (own_slice_len with "Hcap") as %Hlen'.
+  simpl in Hlen'.
+  iExists (take (uint.nat m - uint.nat s.(slice.len_f))%nat vs').
+  iDestruct (own_slice_split_all n with "Hs") as "[Hs1 Hs2]";
+    [ word | ].
+  iDestruct (own_slice_split_all (word.sub m s.(slice.len_f)) with "Hcap") as "[Hvs' Hcap']".
+  { simpl. word. }
+  simpl.
+  iSplitL "Hs1".
+  { iFrame. }
+  iSplitL "Hs2 Hvs'".
+  {
+    iApply (own_slice_split s.(slice.len_f)).
+    { word. }
+    iSplitL "Hs2".
+    { iExactEq "Hs2".
+      f_equal.
+      rewrite -> take_app_ge; len.
+      match goal with
+      | |- context[_ ++ take ?n _] => replace n with 0%nat by word
+      end.
+      rewrite take_0 app_nil_r //.
+    }
+
+    rewrite -> drop_app_le by len.
+    rewrite drop_drop.
+    rewrite -> drop_ge by len.
+    rewrite app_nil_l.
+    replace (uint.nat (word.sub m (slice.len_f s))) with
+      (uint.nat m - uint.nat (slice.len_f s))%nat by word.
+    set (k := (uint.nat m - uint.nat (slice.len_f s))%nat).
+
+    rewrite own_slice_unseal /own_slice_def /=.
+    iDestruct "Hvs'" as "[Hvs' %]".
+    iSplit.
+    2: {
+      iPureIntro; move: Hlen'; len.
+    }
+    change (uint.Z (W64 0)) with 0.
+    rewrite Z.mul_0_r.
+    iExactEq "Hvs'".
+    rewrite loc_add_0 //.
+  }
+  iSplit.
+  { iPureIntro; move: Hlen'; len. }
+  iExists (drop (uint.nat (word.sub m (slice.len_f s))) vs').
+  rewrite /slice.slice_f /=.
+  rewrite !loc_add_assoc -!Z.mul_add_distr_l.
+  iExactEq "Hcap'".
+  repeat (f_equal; try word).
+
+  (* FIXME: automate these simplifications that were helpful to see the proof *)
+  (*
+  replace (word.sub (word.sub (slice.cap_f s) (slice.len_f s)) (word.sub m (slice.len_f s))) with
+    (word.sub s.(slice.cap_f) m) by word.
+  replace (word.sub (word.sub (slice.cap_f s) n) (word.sub m n))
+            with (word.sub s.(slice.cap_f) m) by word.
+  replace (uint.Z n + uint.Z (word.sub m n)) with
+    (uint.Z m) by word.
+  replace (uint.Z (slice.len_f s) + uint.Z (word.sub m (slice.len_f s))) with
+    (uint.Z m) by word.
+
+  iDestruct (own_slice_split (word.sub s.(slice.cap_f) s.(slice.len_f)) with "Hcap'") as "[_ Hcap]".
+  { word. }
+  rewrite /slice.slice_f /=.
+  rewrite !loc_add_assoc -!Z.mul_add_distr_l.
+  replace (uint.nat (word.sub m s.(slice.len_f))) with (uint.nat m - uint.nat s.(slice.len_f))%nat by word.
+  replace (uint.nat (word.sub s.(slice.cap_f) s.(slice.len_f))) with (uint.nat s.(slice.cap_f) - uint.nat s.(slice.len_f))%nat by word.
+  replace (uint.Z n + uint.Z (word.sub m n)) with (uint.Z m) by word.
+  rewrite drop_drop.
+  replace (uint.nat m - uint.nat (slice.len_f s) +
+     (uint.nat (slice.cap_f s) -
+        uint.nat (slice.len_f s) -
+        (uint.nat m -
+           uint.nat (slice.len_f s))))%nat with
+    (uint.nat s.(slice.cap_f) - uint.nat s.(slice.len_f))%nat by word.
+  iExists (drop (uint.nat (slice.cap_f s) -
+                   uint.nat (slice.len_f s))
+             vs').
+*)
 Qed.
 
 Lemma wp_slice_for_range {stk E} sl dq (vs : list V) (body : val) Φ :
@@ -561,7 +1044,7 @@ Lemma wp_load_slice_elem s (i: w64) (vs: list V) dq v :
     ![t] #(slice.elem_ref_f s t i)
   {{{ RET #v; s ↦*{dq} vs }}}.
 Proof.
-  iIntros (Φ) "[Hs %Hlookup] HΦ".
+  wp_start_folded as "[Hs %Hlookup]".
   iDestruct (own_slice_elem_acc with "Hs") as "[Hv Hs]"; [ by eauto | ].
   (* NOTE: cannot use [wp_load] because we need to strip a later *)
   wp_apply (wp_load_ty with "Hv"). iIntros "Hv".
@@ -576,7 +1059,7 @@ Lemma wp_store_slice_elem s (i: w64) (vs: list V) (v': V) :
     store_ty t #(slice.elem_ref_f s t i) #v'
   {{{ RET #(); s ↦* (<[uint.nat i := v']> vs) }}}.
 Proof.
-  iIntros (Φ) "[Hs %bound] HΦ".
+  wp_start_folded as "[Hs %bound]".
   list_elem vs i as v.
   iDestruct (own_slice_elem_acc with "Hs") as "[Hv Hs]"; [ by eauto | ].
   (* NOTE: cannot use [wp_store] because we need to strip a later *)
@@ -584,6 +1067,118 @@ Proof.
   iApply "HΦ".
   iDestruct ("Hs" with "Hv") as "Hs".
   iFrame.
+Qed.
+
+(** slice.copy copies as much as possible (the smaller of len(s) and len(s2)) and returns
+the number of bytes copied. See https://pkg.go.dev/builtin#copy.
+
+Use [take_ge] and [drop_ge] to simplify the resulting list expression.
+ *)
+Lemma wp_slice_copy (s: slice.t) (vs: list V) (s2: slice.t) (vs': list V) dq :
+  {{{ s ↦* vs ∗ s2 ↦*{dq} vs' }}}
+    slice.copy t #s #s2
+  {{{ (n: w64), RET #n; ⌜uint.nat n = Nat.min (length vs) (length vs')⌝ ∗
+                          s ↦* (take (length vs) vs' ++ drop (length vs') vs) ∗
+                          s2 ↦*{dq} vs' }}}.
+Proof.
+  wp_start as "(Hs1 & Hs2)".
+  wp_call.
+  wp_auto.
+  iDestruct (own_slice_len with "Hs1") as %Hlen1.
+  iDestruct (own_slice_len with "Hs2") as %Hlen2.
+  iAssert (∃ (i:w64),
+      "Hs1" ∷ s ↦* (take (uint.nat i) vs' ++ drop (uint.nat i) vs) ∗
+      "Hs2" ∷ s2 ↦*{dq} vs' ∗
+      "i" ∷ i_ptr ↦ i ∗
+      "%" ∷ ⌜uint.Z i ≤ Z.min (uint.Z s.(slice.len_f)) (uint.Z s2.(slice.len_f))⌝
+    )%I with "[Hs1 Hs2 i]" as "IH".
+  { iFrame. word. }
+  wp_for "IH".
+  match goal with
+  | |- context[bool_decide ?P] => destruct (bool_decide_reflect P); wp_auto
+  end.
+  - match goal with
+    | |- context[bool_decide ?P] => destruct (bool_decide_reflect P)
+    end.
+    { rewrite decide_True //; wp_auto.
+      list_elem vs' i as y.
+      wp_apply (wp_load_slice_elem with "[$Hs2]") as "Hs2".
+      { eauto. }
+      wp_apply (wp_store_slice_elem with "[$Hs1]") as "Hs1".
+      { len. }
+      wp_for_post.
+      iFrame.
+      replace (uint.nat (word.add i (W64 1))) with
+        (S (uint.nat i)) by word.
+      iSplit; [ | word ].
+      iExactEq "Hs1".
+      rewrite /named.
+      f_equal.
+      (* TODO: automate list simplification for take/drop/app? *)
+      rewrite -> insert_take_drop by len.
+      rewrite -> take_app_le, -> drop_app_ge by len.
+      rewrite take_take drop_drop.
+      rewrite -> Nat.min_l by auto.
+      erewrite take_S_r; eauto.
+      rewrite -app_assoc /=.
+      rewrite -> length_take_le by word.
+      repeat (f_equal; try word). }
+    rewrite decide_False.
+    2: { inv 1. }
+    rewrite decide_True //.
+    wp_auto.
+    assert (i = slice.len_f s2) by word; subst i.
+    iApply "HΦ".
+    iSplit; [ word | ].
+    iFrame "Hs2".
+    rewrite -> !take_ge by word.
+    iExactEq "Hs1".
+    repeat (f_equal; try word).
+  - rewrite decide_False.
+    2: { inv 1. }
+    rewrite decide_True //.
+    wp_auto.
+    assert (i = slice.len_f s) by word; subst i.
+    iApply "HΦ".
+    iSplit; [ word | ].
+    iFrame "Hs2".
+    rewrite -> !drop_ge, !app_nil_r by word.
+    iExactEq "Hs1".
+    repeat (f_equal; try word).
+Qed.
+
+Lemma own_slice_update_to_dfrac dq (s: slice.t) (vs: list V) :
+  ✓dq →
+  s ↦* vs ⊢ |==> s ↦*{dq} vs.
+Proof.
+  iIntros (Hvalid) "Hs".
+  iMod (dfractional_update_to_dfrac (λ dq, s ↦*{dq} vs) with "Hs") as "$"; auto.
+Qed.
+
+Lemma own_slice_zero_size (s: slice.t) (vs: list V) dq :
+  go_type_size t = 0%nat →
+  length vs = uint.nat (slice.len_f s) →
+  uint.Z s.(slice.len_f) ≤ uint.Z s.(slice.cap_f) →
+  ⊢ s ↦*{dq} vs.
+Proof using IntoValTyped0.
+  intros Hz Hlen Hwf.
+  rewrite own_slice_unseal /own_slice_def.
+  iSplit; [ | auto ].
+  iApply big_sepL_intro.
+  iIntros "!> % % %Hget".
+  iApply (typed_pointsto_zero_size (t:=t)); auto.
+Qed.
+
+Lemma own_slice_cap_zero_size (s: slice.t) :
+  go_type_size t = 0%nat →
+  uint.Z s.(slice.len_f) ≤ uint.Z s.(slice.cap_f) →
+  ⊢ own_slice_cap V s.
+Proof using IntoValTyped0.
+  intros Hz Hwf.
+  rewrite own_slice_cap_unseal /own_slice_cap_def.
+  iSplit; [ auto | ].
+  iExists (replicate (uint.nat (word.sub (slice.cap_f s) (slice.len_f s))) (default_val V)).
+  iApply own_slice_zero_size; simpl; auto; len.
 Qed.
 
 Lemma wp_slice_append (s: slice.t) (vs: list V) (s2: slice.t) (vs': list V) dq :
@@ -595,17 +1190,97 @@ Proof.
   iIntros (Φ) "(Hs & Hcap & Hs2) HΦ".
   wp_call.
   iDestruct (own_slice_len with "Hs") as %Hs.
+  iDestruct (own_slice_len with "Hs2") as %Hs2.
+  iDestruct (own_slice_wf with "Hs") as %Hwf1.
+  iDestruct (own_slice_wf with "Hs2") as %Hwf2.
+  wp_apply wp_sum_assume_no_overflow as "%Hoverflow".
   match goal with
   | |- context[bool_decide ?P] =>
       destruct (bool_decide_reflect P); wp_auto
   end.
-  - admit. (* TODO: slice.slice reasoning, going into capacity *)
-  - wp_apply (wp_ArbitraryInt).
-    iIntros (x). wp_auto.
-    wp_apply wp_slice_make2. iIntros (s') "[Hs_new Hnew_cap]".
+  - wp_pure.
+    { word. }
+    match goal with
+    | |- context[slice.slice_f _ _ ?n ?m] =>
+        iDestruct (own_slice_slice_into_capacity n m with "[$Hs $Hcap]") as
+        (vs'') "(Hs & Hs_new & Hcap)"; [ word | ]
+    end.
     wp_auto.
-    admit. (* TODO: need wp for slice.copy *)
-Admitted.
+    rewrite take_0 drop_0.
+    iClear "Hs". (* empty *)
+    iDestruct (own_slice_len with "Hs_new") as %Hlen.
+    simpl in Hlen; autorewrite with len in Hlen.
+    assert (length vs'' = uint.nat s2.(slice.len_f)) by (move: Hlen; word).
+    wp_apply (wp_slice_slice_with_cap with "[$Hs_new $Hcap]").
+    { iPureIntro; simpl; by len. }
+    iIntros "(Hs_new1 & Hs_new2 & Hs_new_cap)".
+    rewrite -> !slice_f_slice_f by word.
+    rewrite !word.add_0_l.
+    wp_apply (wp_slice_copy with "[$Hs_new2 $Hs2]").
+    autorewrite with len.
+    rewrite -> !Nat.min_l by word.
+    iIntros (n) "(%Hn & Hs_new2 & Hs2)".
+    rewrite -> drop_ge, app_nil_r by len.
+    wp_pures.
+    iApply "HΦ".
+    iFrame "Hs2".
+    iSplitL "Hs_new1 Hs_new2".
+    { iDestruct (own_slice_combine s.(slice.len_f) with "Hs_new1 Hs_new2") as "Hs_new".
+      { len. }
+      rewrite -> !take_app_le, !take_ge by word.
+      iFrame "Hs_new".
+    }
+    iApply (own_slice_cap_slice_f_change_first with "Hs_new_cap").
+    move: l; word.
+  - wp_apply (wp_ArbitraryInt) as "%x".
+    wp_apply wp_sum_assume_no_overflow as "%Hoverflow2".
+    wp_apply wp_slice_make3.
+    { move: Hoverflow2; word. }
+    iIntros (sl) "(Hnew & Hnew_cap & %Hcap)".
+    iDestruct (own_slice_wf with "Hnew") as %Hsl_wf.
+    iDestruct (own_slice_len with "Hnew") as %Hsl_len.
+    autorewrite with len in Hsl_len.
+    assert (word.add (slice.len_f s) (slice.len_f s2) = slice.len_f sl) as Hsl_len'.
+    { apply word.unsigned_inj.
+      move: Hsl_len; word. }
+    wp_pures.
+    wp_apply (wp_slice_copy with "[$Hnew $Hs]").
+    autorewrite with len.
+    rewrite -> !Nat.min_r by word.
+    iIntros (n') "(%Hn' & Hnew & Hs)".
+    rewrite -> take_ge by len.
+    rewrite drop_replicate.
+    wp_pures.
+    wp_apply (wp_slice_slice_with_cap with "[$Hnew $Hnew_cap]").
+    { len. }
+    iIntros "(Hnew1 & Hnew2 & Hnew_cap)".
+    wp_apply (wp_slice_copy with "[$Hnew2 $Hs2]").
+    autorewrite with len.
+    rewrite -> !Nat.min_r by word.
+    iIntros (n'') "(%Hn'' & Hnew2 & Hs2)".
+    rewrite -> !drop_ge, app_nil_r by len.
+    rewrite -> !take_app_le, !take_ge by word.
+    wp_pures.
+    iApply "HΦ".
+    iFrame "Hs2".
+    iSplitL "Hnew1 Hnew2".
+    {
+      iDestruct (own_slice_combine with "Hnew1 Hnew2") as "Hnew".
+      { len. }
+      iDestruct (own_slice_len with "Hnew") as %Hlen.
+      simpl in Hlen.
+      autorewrite with len in Hlen.
+      iExactEq "Hnew".
+      f_equal.
+      rewrite {2}(slice_slice_trivial sl (t:=t)).
+      f_equal.
+      word.
+    }
+    iEval (rewrite (slice_slice_trivial sl (t:=t))).
+    rewrite Hsl_len'.
+    iApply (own_slice_cap_slice_f_change_first with "Hnew_cap").
+    word.
+Qed.
 
 End wps.
 
